rocq-osiris/theories/test/record_test.v
@@ -46,8 +46,6 @@ Section verification.
       ▷ @ownRecord Σ _ τ[Z;Z] r 1 t (x0, y) -∗
       imp m {{ λ (_ : unit), @ownRecord Σ _ τ[Z;Z] r 1 t (x, y) }}.
 
-  Record point : Type := { x : int; y : int }.
-
   Definition eupdate_x := EAnonFun __fun2.
 
   Lemma imp_update_x η :
@@ -81,9 +79,7 @@ Section verification.
       iApply imp_evals_cons. imp_arith.
       iApply imp_evals_singleton. imp_arith. }
 
-    iIntros (r) "H /=". fold eval_sitems.
-    iDestruct "H" as "(% & Hown & Heq)".
-    destruct xs. iDestruct "Heq" as "(-> & ->)".
+    iIntros (r) "(% & % & Hown & (-> & ->))".
 
     iApply (imp_sitems_let (A:=val)).
     { iApply imp_length. }
@@ -99,3 +95,169 @@ Section verification.
   Qed.
 
 End verification.
+
+From osiris.logic Require Import big_opLZ.
+
+Section encoded_fields.
+
+  Context `{!osirisGS Σ}.
+
+  Hypothesis Hmax : 2 ≤ max_array_length.
+
+  Record point : Type := { x : Z; y : Z }.
+
+  Definition ownPoint (r : record) (qp : Qp) (xs : point) : iProp Σ :=
+    (∃ ls, isBlockLocs r ls ∗ r⤇{#qp} Mut ∗
+          [∗ listZ] l;v ∈ ls; [ #xs.(x); #xs.(y)], l ↦{#qp} v)%I.
+
+  Instance name' r p : fractional.Fractional (λ qp, ownPoint r qp p). admit. Admitted.
+
+  Instance name r qp p : fractional.AsFractional (ownPoint r qp p) (λ qp, ownPoint r qp p) qp.
+  Proof.
+    constructor. reflexivity. apply _.
+  Qed.
+
+  Definition point_length_spec r (m : microvx) : iProp Σ :=
+    ∀ qp (p : point),
+      ▷ ownPoint r qp p -∗
+      imp m {{ λ (i : Z), ⌜i = (p.(x) * p.(x) + p.(y) * p.(y))%Z⌝ ∗ ownPoint r qp p }}.
+
+  Definition point_update_x_spec r x (m : microvx) : iProp Σ :=
+    ∀ (p : point),
+      ▷ ownPoint r 1 p -∗
+      imp m {{ λ (_ : unit), ownPoint r 1 {| x := x; y:=p.(y) |} }}.
+
+
+  Lemma ownRecord_ownPoint r qp (x y : Z) :
+    ownRecord (τ:=τ[Z;Z]) r qp Mut (x, y) -∗
+    ownPoint r qp {| x:=x; y:=y |}.
+  Proof.
+    iIntros "(% & Hblock & Htag & Hown)".
+    iFrame.
+  Qed.
+
+  Lemma ownPoint_ownRecord r qp (x y : Z) :
+    ownPoint r qp {| x:=x; y:=y |} -∗
+    ownRecord (τ:=τ[Z;Z]) r qp Mut (x, y).
+  Proof.
+    iIntros "(% & Hblock & Htag & Hown)".
+    iFrame.
+  Qed.
+
+  Lemma imp_point {η E Ψ ζ} e1 e2 (Φs : τ[Z;Z] -#> iProp Σ) :
+    impure E (evals η [e1; e2]) Ψ ζ Φs -∗
+    impure E (eval η (ERecord Mut [e1; e2])) Ψ ζ (λ r, ∃ x y, ownPoint r 1 {| x := x; y := y |} ∗ Φs x y)%I.
+  Proof.
+    iIntros "Hes".
+    iApply (imp_wand with "[-]").
+    { iApply (imp_ERecord with "Hes"). assumption. }
+    iIntros (r) "(% & % & Hrecord & $)".
+    iApply (ownRecord_ownPoint with "Hrecord").
+  Qed.
+
+  Lemma imp_point_x {η : env} {E : coPset} {Ψ : iEff Σ} {ζ : exn → iProp Σ}
+    (r : record) (dq : Qp) (p : point) (e : expr) :
+    ▷ ownPoint r dq p -∗
+    imp eval η e @ E <| Ψ |> ⟨⟨ ζ ⟩⟩ {{ λ r' : record, ⌜r' = r⌝ }} -∗
+    imp eval η (ERecordAccess e 0%Z) @ E <| Ψ |> ⟨⟨ ζ ⟩⟩ {{ λ i : Z, ⌜i = x p⌝ ∗ ownPoint r dq p }}.
+  Proof.
+    iIntros "Hown He".
+    iApply (imp_wand with "[-]").
+    { iApply (imp_ERecordAccess (τ:=τ[Z;Z]) _ 0 with "[Hown] He").
+      split; simpl; lia.
+      iApply (ownPoint_ownRecord with "Hown"). }
+    iIntros (x) "(-> & $)". iPureIntro. reflexivity.
+  Qed.
+
+  Lemma imp_point_y {η : env} {E : coPset} {Ψ : iEff Σ} {ζ : exn → iProp Σ}
+    (r : record) (dq : Qp) (p : point) (e : expr) :
+    ▷ ownPoint r dq p -∗
+    imp eval η e @ E <| Ψ |> ⟨⟨ ζ ⟩⟩ {{ λ r' : record, ⌜r' = r⌝ }} -∗
+    imp eval η (ERecordAccess e 1%Z) @ E <| Ψ |> ⟨⟨ ζ ⟩⟩ {{ λ i : Z, ⌜i = y p⌝ ∗ ownPoint r dq p }}.
+  Proof.
+    iIntros "Hown He".
+    iApply (imp_wand with "[-]").
+    { iApply (imp_ERecordAccess (τ:=τ[Z;Z]) with "[Hown] He").
+      split; simpl; lia.
+      iApply (ownPoint_ownRecord with "Hown"). }
+    iIntros (x) "(-> & $)". iPureIntro. reflexivity.
+  Qed.
+
+  Lemma point_update_x {η E Ψ ζ} (r : record) p e1 e2 (Φ : Z → iProp Σ) :
+    ▷ ownPoint r 1 p -∗
+    impure E (eval η e1) Ψ ζ (λ r', ⌜r' = r⌝) -∗
+    impure E (eval η e2) Ψ ζ Φ -∗
+    impure E (eval η (ERecordSet e1 0 e2)) Ψ ζ (λ (_ : ()), ∃ x, Φ x ∗ ownPoint r 1 {| x:=x; y:=p.(y) |})%I.
+  Proof.
+    iIntros "Hown He1 He2".
+    iApply (imp_wand with "[-]").
+    { iApply (imp_ERecordSet (τ:=τ[Z;Z]) with "[Hown] He1 [He2]").
+      { split; simpl; lia. }
+      iApply (ownPoint_ownRecord with "Hown").
+      iApply "He2". }
+    iIntros ([]) "(%x & $ & $)".
+  Qed.
+
+  Lemma imp_point_length η :
+    ⊢ imp (eval η elength) {{ λ length, □ iSpec τ[record] length point_length_spec }}.
+  Proof.
+    iApply imp_EAnon_pers.
+    iIntros "!>" (r qp p) "Hown".
+
+    iApply imp_please; iNext.
+
+    (* Goal: [(v.x * v.x) + (v.y * v.y)] *)
+    imp_arith reading "Hown".
+    (* All remaining subgoals are of the form [v.x] *)
+    - iApply (imp_point_x with "Hown"); imp_path.
+    - iApply (imp_point_x with "Hown"); imp_path.
+    - iApply (imp_point_y with "Hown"); imp_path.
+    - iApply (imp_point_y with "Hown"); imp_path.
+  Qed.
+
+  Lemma imp_point_update_x η :
+    ⊢ imp (eval η eupdate_x) {{ λ update_x, □ iSpec τ[record; Z] update_x point_update_x_spec }}.
+  Proof.
+    iApply imp_EAnon_pers.
+    iIntros "!>" (r x p) "Hown".
+    iApply imp_please; iNext.
+
+    iApply imp_mono_val; last first.
+    { iApply (point_update_x with "Hown"). imp_path. imp_path. }
+    iIntros ([]) "(% & -> & $)".
+  Qed.
+
+
+  Lemma point_module_proof η :
+    2 ≤ max_array_length →
+    ⊢ imp (eval_mexpr η __main)
+      {{ context
+           [ var_spec "length" (λ length, iSpec τ[record] length point_length_spec);
+             var_spec "update_x" (λ update, iSpec τ[record;Z] update point_update_x_spec) ]
+           {[ "vec"; "length"; "update_x" ]} }}.
+  Proof.
+    intros Hmax_array.
+    iApply imp_module.
+
+    iApply (imp_sitems_let (A:=record)).
+    { iApply imp_point.
+      iApply imp_evals_cons. imp_arith.
+      iApply imp_evals_singleton. imp_arith. }
+
+    iIntros (r) "(% & % & Hown & (-> & ->))".
+
+    iApply (imp_sitems_let (A:=val)).
+    { iApply imp_point_length. }
+
+    iIntros (length) "#Hlength".
+
+    iApply (imp_sitems_let (A:=val)).
+    { iApply imp_point_update_x. }
+
+    iIntros (update_x) "#Hupdate_x".
+    iApply imp_sitems_nil.
+    iFrame "#". simpl. auto.
+  Qed.
+
+
+End encoded_fields.
